@prefix cx-common: <https://w3id.org/catenax/ontology/common#> .
@prefix cx-core: <https://w3id.org/catenax/ontology/core#> .
@prefix dc: <http://purl.org/dc/elements/1.1/> .
@prefix owl: <http://www.w3.org/2002/07/owl#> .
@prefix rdf: <http://www.w3.org/1999/02/22-rdf-syntax-ns#> .
@prefix rdfs: <http://www.w3.org/2000/01/rdf-schema#> .
@prefix sh: <http://www.w3.org/ns/shacl#> .
@prefix xsd: <http://www.w3.org/2001/XMLSchema#> .

dc:creator a owl:AnnotationProperty .

dc:date a owl:AnnotationProperty .

dc:description a owl:AnnotationProperty .

dc:title a owl:AnnotationProperty .

sh:shapesGraph a owl:DatatypeProperty ;
    rdfs:label "shapes graph"@en ;
    rdfs:comment "This property refers to a SHACL expression in which the RDF data Contraints are defined. In particular, the structure of the identifiers."@en ;
    rdfs:domain cx-common:Asset ;
    rdfs:range xsd:anyURI .

<https://w3id.org/catenax/ontology/common> a owl:Ontology ;
    dc:contributor "[@drcgjung](https://github.com/drcgjung) , [@obalandi](https://github.com/obalandi)" ;
    dc:creator "[@ZazraltMagic](https://github.com/ZazraltMagic)" ;
    dc:date "2023-05-23"^^xsd:date ;
    dc:description "The common ontology describes the Dataspace connectors in detail. On the one hand, this includes the information from which Catena-X business partner the connectors are deployed. On the other hand, with which contracts which assets provide the connectors."@en ;
    dc:title "Common Ontology" ;
    owl:imports <file:core_ontology.ttl> ;
    owl:versionInfo "1.9.4" .

cx-common:authenticatedResource a rdfs:DatatypeProperty ;
    rdfs:label "Authenticated Resource"@en ;
    rdfs:comment "An resource that requires authentication."@en ;
    rdfs:domain cx-common:Asset ;
    rdfs:range xsd:anyURI .

cx-common:authenticationCode a owl:DatatypeProperty ;
    rdfs:label "authentication code"@en ;
    rdfs:comment "An authentication code under which authentication information are transmitted." ;
    rdfs:domain cx-common:Asset ;
    rdfs:range xsd:string ;
    rdfs:subPropertyOf cx-common:authenticationInformation .

cx-common:authenticationKey a owl:DatatypeProperty ;
    rdfs:label "authentication key"@en ;
    rdfs:comment "An authentication key which encodes some authentication proof." ;
    rdfs:domain cx-common:Asset ;
    rdfs:range xsd:string ;
    rdfs:subPropertyOf cx-common:authenticationInformation .

cx-common:contentType a owl:DatatypeProperty ;
    rdfs:label "content type"@en ;
    rdfs:comment "This property describes in which format the data will be output, i.e. XML or JSON."@en ;
    rdfs:domain cx-common:Asset ;
    rdfs:range xsd:string ;
    rdfs:subPropertyOf owl:topDataProperty .

cx-common:description a owl:DatatypeProperty ;
    rdfs:label "description"@en ;
    rdfs:comment "This property contains description of asset."@en ;
    rdfs:domain cx-common:Asset ;
    rdfs:range xsd:string ;
    rdfs:subPropertyOf owl:topDataProperty .

cx-common:distributionMode a owl:DatatypeProperty ;
    rdfs:label "Distribution Mode"@en ;
    rdfs:comment "The skill may only be invoked local to the computing environment of the provider."@en ;
    rdfs:domain cx-common:Asset ;
    rdfs:range xsd:string .

cx-common:hasDataspaceConnector a owl:ObjectProperty ;
    rdfs:label "has Dataspace Connector"@en ;
    rdfs:comment "This property describes which connectors belong to which business partners."@en ;
    rdfs:domain cx-common:BusinessPartner ;
    rdfs:range cx-common:DataspaceConnector ;
    rdfs:subPropertyOf owl:topObjectProperty .

cx-common:id a owl:DatatypeProperty ;
    rdfs:label "id"@en ;
    rdfs:comment "This property contains unique identifier of Bussiness Partner/Connector/Asset."@en ;
    rdfs:domain cx-common:Asset ;
    rdfs:range xsd:string ;
    rdfs:subPropertyOf owl:topDataProperty .

cx-common:implementsProtocol a owl:DatatypeProperty ;
    rdfs:label "implements protocol"@en ;
    rdfs:comment "This property refers to the network protocol implemented by the asset."@en ;
    rdfs:domain cx-common:Asset ;
    rdfs:range xsd:string ;
    rdfs:subPropertyOf owl:topDataProperty .

cx-common:isFederated a owl:DatatypeProperty ;
    rdfs:label "is federated"@en ;
    rdfs:comment "If this property is set to true, it means that this connector will federate with other connectors."@en ;
    rdfs:domain cx-common:Asset ;
    rdfs:range xsd:boolean ;
    rdfs:subPropertyOf owl:topDataProperty .

cx-common:name a owl:DatatypeProperty ;
    rdfs:label "name"@en ;
    rdfs:comment "This property contains name of asset."@en ;
    rdfs:domain cx-common:Asset ;
    rdfs:range xsd:string ;
    rdfs:subPropertyOf owl:topDataProperty .

cx-common:offers a owl:ObjectProperty ;
    rdfs:label "offers"@en ;
    rdfs:comment "This property refers to the offered assets."@en ;
    rdfs:domain cx-common:DataspaceConnector ;
    rdfs:range cx-common:Asset ;
    rdfs:subPropertyOf owl:topObjectProperty .

cx-common:publishedUnderContract a owl:DatatypeProperty ;
    rdfs:label "published under contract"@en ;
    rdfs:comment "This property refers to the contract associated with the asset."@en ;
    rdfs:domain cx-common:Asset ;
    rdfs:range xsd:string ;
    rdfs:subPropertyOf owl:topDataProperty .

cx-common:satisfiesRole a owl:DatatypeProperty ;
    rdfs:label "satisfies role"@en ;
    rdfs:comment "Use Case Role IRI."@en ;
    rdfs:domain cx-common:Asset ;
    rdfs:range xsd:anyURI ;
    rdfs:subPropertyOf owl:topDataProperty .

cx-common:url a owl:DatatypeProperty ;
    rdfs:label "url"@en ;
    rdfs:comment ""@en ;
    rdfs:domain cx-common:DataspaceConnector ;
    rdfs:range xsd:anyURI ;
    rdfs:subPropertyOf owl:topDataProperty .

cx-common:version a owl:DatatypeProperty ;
    rdfs:label "version"@en ;
    rdfs:comment "Version of the asset."@en ;
    rdfs:domain cx-common:Asset ;
    rdfs:range xsd:string ;
    rdfs:subPropertyOf owl:topDataProperty .

<https://w3id.org/catenax/ontology/core> a owl:Ontology ;
    dc:creator "[@obalandi](https://github.com/obalandi)" ;
    dc:date "2023-05-05"^^xsd:date ;
    dc:description "The Catena-X core ontology is an activity-centric top-level ontology and enables the design of domain ontologies on the basis of main classes." ;
    dc:title "Core Ontology" ;
    owl:versionInfo "1.9.4" .

cx-core:city a owl:DatatypeProperty ;
    rdfs:label "city"@en ;
    rdfs:comment "City name of a legal address."@en ;
    rdfs:domain cx-core:Address ;
    rdfs:range xsd:string ;
    rdfs:subPropertyOf owl:topDataProperty .

cx-core:country a owl:DatatypeProperty ;
    rdfs:label "country"@en ;
    rdfs:comment "Country name of a legal address."@en ;
    rdfs:domain cx-core:Address ;
    rdfs:range xsd:string ;
    rdfs:subPropertyOf owl:topDataProperty .

cx-core:describedByConceptualObject a owl:ObjectProperty ;
    rdfs:label "described by conceptual object"@en ;
    rdfs:comment "Inverse of 'describes physical object' property."@en ;
    rdfs:domain cx-core:PhysicalObject ;
    rdfs:range cx-core:ConceptualObject ;
    rdfs:subPropertyOf owl:topObjectProperty ;
    owl:inverseOf cx-core:describesPhysicalObject .

cx-core:endDateTime a owl:DatatypeProperty ;
    rdfs:label "end dateTime"@en ;
    rdfs:comment "End time of the activity."@en ;
    rdfs:domain cx-core:Activity ;
    rdfs:range xsd:dateTime ;
    rdfs:subPropertyOf owl:topDataProperty .

cx-core:hasAddress a owl:ObjectProperty ;
    rdfs:label "has address"@en ;
    rdfs:comment "Inverse of 'describes physical object' property."@en ;
    rdfs:domain cx-core:Place ;
    rdfs:range cx-core:Address ;
    rdfs:subPropertyOf owl:topObjectProperty .

cx-core:hosts a owl:ObjectProperty ;
    rdfs:label "hosts"@en ;
    rdfs:comment "Inverse of 'takes place at' property." ;
    rdfs:domain cx-core:Place ;
    rdfs:range cx-core:Activity ;
    rdfs:subPropertyOf owl:topObjectProperty ;
    owl:inverseOf cx-core:takesPlaceAt .

cx-core:houseNumber a owl:DatatypeProperty ;
    rdfs:label "house number"@en ;
    rdfs:comment "House number of a legal address."@en ;
    rdfs:domain cx-core:Address ;
    rdfs:range xsd:string ;
    rdfs:subPropertyOf owl:topDataProperty .

cx-core:id a owl:DatatypeProperty ;
    rdfs:label "id"@en ;
    rdfs:comment "Unique identification of the exchanged Catena-X objects."@en ;
    rdfs:domain cx-core:Activity,
        cx-core:Actor,
        cx-core:ConceptualObject,
        cx-core:PhysicalObject,
        cx-core:Place ;
    rdfs:range xsd:string ;
    rdfs:subPropertyOf owl:topDataProperty .

cx-core:involvedIn a owl:ObjectProperty ;
    rdfs:label "involved in"@en ;
    rdfs:comment "This property describes in which activity the physical object is involved."@en ;
    rdfs:domain cx-core:ConceptualObject,
        cx-core:PhysicalObject ;
    rdfs:range cx-core:Activity ;
    owl:inverseOf cx-core:refersToConceptualObject,
        cx-core:refersToPhysicalObject .

cx-core:name a owl:DatatypeProperty ;
    rdfs:label "name"@en ;
    rdfs:comment "Global name of an object."@en ;
    rdfs:domain cx-core:Activity,
        cx-core:Actor,
        cx-core:ConceptualObject,
        cx-core:PhysicalObject,
        cx-core:Place ;
    rdfs:range xsd:string ;
    rdfs:subPropertyOf owl:topDataProperty .

cx-core:participatesIn a owl:ObjectProperty ;
    rdfs:label "participates in"@en ;
    rdfs:comment "Inverse of 'has participant' property."@en ;
    rdfs:domain cx-core:Actor ;
    rdfs:range cx-core:Activity ;
    rdfs:subPropertyOf owl:topObjectProperty ;
    owl:inverseOf cx-core:hasParticipant .

cx-core:postalCode a owl:DatatypeProperty ;
    rdfs:label "postal code"@en ;
    rdfs:comment "Postal code of a legal address."@en ;
    rdfs:domain cx-core:Address ;
    rdfs:range xsd:string ;
    rdfs:subPropertyOf owl:topDataProperty .

cx-core:relatedToPlace a owl:ObjectProperty ;
    rdfs:label "related to place."@en ;
    rdfs:comment "This property describes that an actor has a relationship to a particular place, such as reside, own, or manage, etc."@en ;
    rdfs:domain cx-core:Actor ;
    rdfs:range cx-core:Place .

cx-core:startDateTime a owl:DatatypeProperty ;
    rdfs:label "start dateTime"@en ;
    rdfs:comment "Start time of an activity."@en ;
    rdfs:domain cx-core:Activity ;
    rdfs:range xsd:dateTime ;
    rdfs:subPropertyOf owl:topDataProperty .

cx-core:street a owl:DatatypeProperty ;
    rdfs:label "street"@en ;
    rdfs:comment "Street name of alegal address."@en ;
    rdfs:domain cx-core:Address ;
    rdfs:range xsd:string ;
    rdfs:subPropertyOf owl:topDataProperty .

cx-common:BusinessPartner a owl:Class ;
    rdfs:label "Business Partner"@en ;
    rdfs:comment "A Business Partner is a legal entity that is part of the Catena-X network or that stands in a relevant relation to a Catena-X Business Partner."@en ;
    rdfs:subClassOf cx-core:Actor .

cx-core:describesPhysicalObject a owl:ObjectProperty ;
    rdfs:label "describes physical object"@en ;
    rdfs:comment "This property describes that a conceptual object has a descriptive relationship to a physical object."@en ;
    rdfs:domain cx-core:ConceptualObject ;
    rdfs:range cx-core:PhysicalObject ;
    rdfs:subPropertyOf owl:topObjectProperty .

cx-core:hasParticipant a owl:ObjectProperty ;
    rdfs:label "has participant"@en ;
    rdfs:comment "This property describes the active or passive participation of instances of Actors in an Activity."@en ;
    rdfs:domain cx-core:Activity ;
    rdfs:range cx-core:Actor ;
    rdfs:subPropertyOf owl:topObjectProperty .

cx-core:refersToConceptualObject a owl:ObjectProperty ;
    rdfs:label "refers to conceptual object."@en ;
    rdfs:comment "This property refers to actively or passively used conceptual objects in an Activity."@en ;
    rdfs:domain cx-core:Activity ;
    rdfs:range cx-core:ConceptualObject ;
    rdfs:subPropertyOf owl:topObjectProperty .

cx-core:refersToPhysicalObject a owl:ObjectProperty ;
    rdfs:label "refers to physical object."@en ;
    rdfs:comment "This property refers to actively or passively used physical objects in an Activity."@en ;
    rdfs:domain cx-core:Activity ;
    rdfs:range cx-core:PhysicalObject ;
    rdfs:subPropertyOf owl:topObjectProperty .

cx-core:takesPlaceAt a owl:ObjectProperty ;
    rdfs:label "takes place at"@en ;
    rdfs:comment "This property describes the spatial location of an activity."@en ;
    rdfs:domain cx-core:Activity ;
    rdfs:range cx-core:Place .

cx-common:Application a owl:Class ;
    rdfs:label "Application"@en ;
    rdfs:comment "An application defines a coded software that fulfills a specific purpose."@en .

cx-common:authenticationInformation a owl:DatatypeProperty ;
    rdfs:label "authentication information"@en ;
    rdfs:comment "Base property for all authentication informations." ;
    rdfs:domain cx-common:Asset ;
    rdfs:range xsd:string ;
    rdfs:subPropertyOf owl:topDataProperty .

cx-common:DataspaceConnector a owl:Class ;
    rdfs:label "Dataspace Connector"@en ;
    rdfs:comment "Dataspace Connector is an interface based on the Eclipse Dataspace Connector technology. A Dataspace Connector makes various assets available through contracts. A contract describes with which policy which asset can be provided."@en ;
    rdfs:seeAlso <https://projects.eclipse.org/proposals/eclipse-dataspace-connector> ;
    rdfs:subClassOf cx-common:Application .

cx-core:Actor a owl:Class ;
    rdfs:label "Actor" ;
    rdfs:comment "This class comprises organization or people, either individually or in groups, who have the potential to perform intentional actions of kinds for which someone may be held responsible."@en .

cx-core:Address a owl:Class ;
    rdfs:label "Address"@en ;
    rdfs:comment "This class describes the legal address of places."@en ;
    rdfs:subClassOf cx-core:ConceptualObject .

cx-core:PhysicalObject a owl:Class ;
    rdfs:label "Physical Object"@en ;
    rdfs:comment "This class includes objects of a material nature, which are documentation units and have physical boundaries."@en .

cx-core:Place a owl:Class ;
    rdfs:label "Place"@en ;
    rdfs:comment "The class Place is determined by reference to the position of objects such as buildings, cities, or special geographic markers."@en .

cx-core:ConceptualObject a owl:Class ;
    rdfs:label "Conceptual Object"@en ;
    rdfs:comment "This class includes non-material products, human-produced data related to physical objects. The production of such information may have been supported by the use of technical tools."@en .

cx-core:Activity a owl:Class ;
    rdfs:label "Activity"@en ;
    rdfs:comment "This class comprises actions intentionally carried out by instances of Actor that result in changes of state in physical and conceptual objects."@en ;
    owl:disjointUnionOf ( cx-core:Actor cx-core:Address cx-core:ConceptualObject cx-core:PhysicalObject cx-core:Place ) .

cx-common:Asset a owl:Class ;
    rdfs:label "Asset"@en ;
    rdfs:comment "The Asset class describes the provision via a repository of a specific set of data for a specific purpose."@en ;
    rdfs:subClassOf cx-common:Application .

